lntls.v
@@ -121,6 +121,125 @@ Undo 2.
 
 Check gen_swapL.
 
+(* alternative proof using step lemma *)
+Lemma gen_swapL_step_pr: forall V ps concl 
+  (last_rule rules : rls (list (rel (list (PropF V)) * dir))),
+  last_rule = nsrule (seqrule (@princrule V)) ->
+  gen_swapL_step last_rule rules ps concl.
+Proof.  intros until 0.  unfold gen_swapL_step.
+intros lreq nsr drs acm rs. subst.
+
+inversion nsr as [? ? ? K ? sppc mnsp nsc].
+unfold nsext in nsc.
+unfold can_gen_swapL.   intros until 0. intros pp ss.
+unfold nsext in pp.
+
+apply partition_2_2 in pp.
+remember (Γ1 ++ Γ3 ++ Γ2 ++ Γ4, Δ) as seqe.
+
+decompose [or] pp. 
+
+{ nsright' pp G0 seqe d0 x c0 Ge HeqGe
+  K d ps ps0 inps0 pse K0 drs nsr acm G seq rs. }
+all : revgoals.
+{ nsleft' pp G0 seqe d0 x c0 He HeqHe
+  K d ps ps0 inps0 pse K0 drs nsr acm G seq rs. }
+
+(* now case where move and rule application occur in the same sequent *)
+cE. clear pp. injection H0 as.
+inversion sppc as [? ? ? ? ? ? pr mse se].
+unfold seqext in se.
+subst.  clear nsr. clear sppc.
+destruct c0. 
+injection se as sel ser.
+subst.
+(* do as much as possible for all rules at once *)
+acacD' ; (* gives 10 subgoals *)
+subst ;
+repeat ((list_eq_nc || (pose pr as Qpr ; apply princrule_L_oe in Qpr)) ;
+  sD ; subst ; simpl ; simpl in pr ;
+  try (rewrite app_nil_r) ; try (rewrite app_nil_r in pr)).
+
+(* need to do stage1 pr. to see what next,
+  then stage12ds acm qin1 qin3 pr ...,
+  then all : solve_eqs. to see what next *)
+
+{ stage12altdsL' rs drs acm qin1 qin3 pr ; solve_eqs ;
+rewrite (app_assoc l) ; reflexivity.  }
+
+{ stage12altdsL' rs drs acm qin1 qin3 pr ; solve_eqs ;
+rewrite (app_assoc sel) ; reflexivity.  }
+
+{ stage12altdsL' rs drs acm qin1 qin3 pr. }
+
+{ stage12altdsL' rs drs acm qin1 qin3 pr ; solve_eqs ; reflexivity. }
+
+{ stage12altdsL' rs drs acm qin1 qin3 pr ; solve_eqs. }
+
+{ stage12altdsL' rs drs acm qin1 qin3 pr ; solve_eqs ; 
+rewrite (app_assoc l1) ; rewrite (app_assoc sel) ; reflexivity. }
+
+{ stage12altdsL' rs drs acm qin1 qin3 pr ; solve_eqs ; reflexivity. }
+
+{ stage12altdsL' rs drs acm qin1 qin3 pr ; solve_eqs ;
+rewrite (app_assoc sel1) ; reflexivity. }
+
+{ stage12altdsL' rs drs acm qin1 qin3 pr ; solve_eqs ;
+rewrite (app_assoc l1) ; rewrite (app_assoc sel1) ; reflexivity. }
+
+{ stage12altdsL' rs drs acm qin1 qin3 pr ; solve_eqs ; reflexivity. }
+
+{ stage12altdsL' rs drs acm qin1 qin3 pr ; solve_eqs ;
+rewrite (app_assoc l) ; reflexivity. }
+
+{ stage12altdsL' rs drs acm qin1 qin3 pr ; solve_eqs ;
+rewrite (app_assoc Φ1) ; reflexivity. }
+
+{ stage12altdsL' rs drs acm qin1 qin3 pr ; solve_eqs. }
+
+{ stage12altdsL' rs drs acm qin1 qin3 pr ; solve_eqs ; reflexivity. }
+
+{ stage12altdsL' rs drs acm qin1 qin3 pr ; solve_eqs. }
+
+{ stage12altdsL' rs drs acm qin1 qin3 pr ; solve_eqs. }
+
+{ stage12altdsL' rs drs acm qin1 qin3 pr ; solve_eqs. }
+
+{ stage12altdsL' rs drs acm qin1 qin3 pr ; solve_eqs. }
+
+{ stage12altdsL' rs drs acm qin1 qin3 pr ; solve_eqs. }
+
+{ stage12altdsL' rs drs acm qin1 qin3 pr ; solve_eqs ;
+rewrite (app_assoc l1) ; rewrite (app_assoc Φ1) ; reflexivity. }
+
+Qed.
+
+Check gen_swapL_step_pr.
+
+Lemma gen_swapL': forall (V : Set) ns
+  (D : derrec (nsrule (seqrule (@princrule V))) (fun _ => False) ns),
+  can_gen_swapL (nsrule (seqrule (@princrule V))) ns.
+
+Proof. 
+intro.  intro.  intro.
+eapply derrec_all_ind in D.
+exact D. tauto.
+intros. inversion H. 
+subst.
+pose gen_swapL_step_pr.
+unfold gen_swapL_step in g.
+eapply g. reflexivity. eassumption. assumption. assumption.
+unfold rsub. clear g. 
+intros.  assumption.
+Qed.
+
+
+
+
+
+
+
+
 
 
 
